theories/generic/utp_composite_value.thy
@@ -1,0 +1,297 @@
+(******************************************************************************)
+(* Title: utp/generic/utp_composite_value.thy                                 *)
+(* Author: Frank Zeyda, University of York                                    *)
+(******************************************************************************)
+theory utp_composite_value
+imports "../utp_sorts" utp_abstract_value
+begin
+
+section {* Composite Values *}
+
+subsection {* Data Types *}
+
+text {*
+  The @{text "SetVal"} constructor might need to know about the type of
+  elements the set.
+*}
+
+datatype 'BASIC_VALUE COMPOSITE_VALUE =
+  BasicVal "'BASIC_VALUE" |
+  PairVal "'BASIC_VALUE COMPOSITE_VALUE" "'BASIC_VALUE COMPOSITE_VALUE" |
+  SetVal "'BASIC_VALUE COMPOSITE_VALUE SET"
+
+datatype 'BASIC_TYPE COMPOSITE_TYPE =
+  BasicType "'BASIC_TYPE" |
+  PairType "'BASIC_TYPE COMPOSITE_TYPE" "'BASIC_TYPE COMPOSITE_TYPE" |
+  SetType "'BASIC_TYPE COMPOSITE_TYPE"
+
+subsubsection {* Destructors *}
+
+primrec ValOf ::
+  "'BASIC_VALUE COMPOSITE_VALUE \<Rightarrow> 'BASIC_VALUE" where
+"ValOf (BasicVal v) = v"
+
+primrec PairOf ::
+  "'BASIC_VALUE COMPOSITE_VALUE \<Rightarrow>
+  ('BASIC_VALUE COMPOSITE_VALUE \<times>
+   'BASIC_VALUE COMPOSITE_VALUE)" where
+"PairOf (PairVal v1 v2) = (v1, v2)"
+
+primrec SetOf ::
+  "'BASIC_VALUE COMPOSITE_VALUE \<Rightarrow>
+   'BASIC_VALUE COMPOSITE_VALUE SET" where
+"SetOf (SetVal s) = s"
+
+subsubsection {* Tests *}
+
+primrec IsBasicVal ::
+  "'BASIC_VALUE COMPOSITE_VALUE \<Rightarrow> bool" where
+"IsBasicVal (BasicVal v) = True" |
+"IsBasicVal (PairVal v1 v2) = False" |
+"IsBasicVal (SetVal s) = False"
+
+primrec IsPairVal ::
+  "'BASIC_VALUE COMPOSITE_VALUE \<Rightarrow> bool" where
+"IsPairVal (BasicVal v) = False" |
+"IsPairVal (PairVal v1 v2) = True" |
+"IsPairVal (SetVal s) = False"
+
+primrec IsSetVal ::
+  "'BASIC_VALUE COMPOSITE_VALUE \<Rightarrow> bool" where
+"IsSetVal (BasicVal v) = False" |
+"IsSetVal (PairVal v1 v2) = False" |
+"IsSetVal (SetVal s) = True"
+
+subsubsection {* Abbreviations *}
+
+abbreviation EncSetVal ::
+  "'BASIC_VALUE COMPOSITE_VALUE set \<Rightarrow>
+   'BASIC_VALUE COMPOSITE_VALUE" where
+"EncSetVal vs \<equiv> SetVal (EncSet vs)"
+
+abbreviation DecSetOf ::
+  "'BASIC_VALUE COMPOSITE_VALUE \<Rightarrow>
+   'BASIC_VALUE COMPOSITE_VALUE set" where
+"DecSetOf v \<equiv> DecSet (SetOf v)"
+
+subsection {* Sort Membership *}
+
+instantiation COMPOSITE_VALUE :: (BASIC_SORT) COMPOSITE_SORT
+begin
+definition MkInt_COMPOSITE_VALUE [simp] :
+"MkInt_COMPOSITE_VALUE i = BasicVal (MkInt i)"
+definition DestInt_COMPOSITE_VALUE [simp] :
+"DestInt_COMPOSITE_VALUE v = DestInt (ValOf v)"
+definition IsInt_COMPOSITE_VALUE [simp] :
+"IsInt_COMPOSITE_VALUE v \<longleftrightarrow> (IsBasicVal v) \<and> IsInt (ValOf v)"
+definition MkBool_COMPOSITE_VALUE [simp] :
+"MkBool_COMPOSITE_VALUE b = BasicVal (MkBool b)"
+definition DestBool_COMPOSITE_VALUE [simp] :
+"DestBool_COMPOSITE_VALUE v = DestBool (ValOf v)"
+definition IsBool_COMPOSITE_VALUE [simp] :
+"IsBool_COMPOSITE_VALUE v \<longleftrightarrow> (IsBasicVal v) \<and> IsBool (ValOf v)"
+definition MkStr_COMPOSITE_VALUE [simp] :
+"MkStr_COMPOSITE_VALUE s = BasicVal (MkStr s)"
+definition DestStr_COMPOSITE_VALUE [simp] :
+"DestStr_COMPOSITE_VALUE v = DestStr (ValOf v)"
+definition IsStr_COMPOSITE_VALUE [simp] :
+"IsStr_COMPOSITE_VALUE v \<longleftrightarrow> (IsBasicVal v) \<and> IsStr (ValOf v)"
+definition MkPair_COMPOSITE_VALUE [simp] :
+"MkPair_COMPOSITE_VALUE v1_v2 = (uncurry PairVal) v1_v2"
+definition DestPair_COMPOSITE_VALUE [simp] :
+"DestPair_COMPOSITE_VALUE v = PairOf v"
+definition IsPair_COMPOSITE_VALUE [simp] :
+"IsPair_COMPOSITE_VALUE v \<longleftrightarrow> IsPairVal v"
+definition MkSet_COMPOSITE_VALUE [simp] :
+"MkSet_COMPOSITE_VALUE vs = EncSetVal vs"
+definition DestSet_COMPOSITE_VALUE [simp] :
+"DestSet_COMPOSITE_VALUE v = DecSetOf v"
+definition IsSet_COMPOSITE_VALUE [simp] :
+"IsSet_COMPOSITE_VALUE v \<longleftrightarrow> IsSetVal v"
+instance
+apply (intro_classes)
+apply (simp_all add: uncurry_def)
+done
+end
+
+subsection {* Lifting Functors *}
+
+fun lift_type_rel_composite ::
+  "('BASIC_VALUE \<Rightarrow> 'BASIC_TYPE \<Rightarrow> bool) \<Rightarrow>
+   ('BASIC_VALUE COMPOSITE_VALUE \<Rightarrow>
+    'BASIC_TYPE COMPOSITE_TYPE \<Rightarrow> bool)"
+  ("(_ \<bowtie> _ :/ _)" [50, 51] 50) where
+"type_rel \<bowtie> (BasicVal v) : (BasicType t) = (type_rel v t)" |
+"type_rel \<bowtie> (BasicVal v) : (PairType t1 t2) = False" |
+"type_rel \<bowtie> (BasicVal v) : (SetType t) = False" |
+"type_rel \<bowtie> (PairVal v1 v2) : (BasicType t) = False" |
+"type_rel \<bowtie> (PairVal v1 v2) : (PairType t1 t2) =
+ ((type_rel \<bowtie> v1 : t1) \<and> (type_rel \<bowtie> v2 : t2))" |
+"type_rel \<bowtie> (PairVal v1 v2) : (SetType t) = False" |
+"type_rel \<bowtie> (SetVal vs) : (BasicType t) = False" |
+"type_rel \<bowtie> (SetVal vs) : (PairType t1 t2) = False" |
+"type_rel \<bowtie> (SetVal vs) : (SetType t) =
+ (\<forall> v \<in> DecSet(vs) . (type_rel) \<bowtie> v : t)"
+
+fun lift_value_ref_composite ::
+  "('BASIC_VALUE \<Rightarrow> 'BASIC_VALUE \<Rightarrow> bool) \<Rightarrow>
+   ('BASIC_VALUE COMPOSITE_VALUE \<Rightarrow>
+    'BASIC_VALUE COMPOSITE_VALUE \<Rightarrow> bool)"
+  ("(_ \<bowtie> _ \<sqsubseteq>/ _)" [50, 51] 50) where
+"value_ref \<bowtie> (BasicVal v) \<sqsubseteq> (BasicVal v') = (value_ref v v')" |
+"value_ref \<bowtie> (BasicVal v) \<sqsubseteq> (PairVal v1' v2') = False" |
+"value_ref \<bowtie> (BasicVal v) \<sqsubseteq> (SetVal vs') = False" |
+"value_ref \<bowtie> (PairVal v1 v2) \<sqsubseteq> (BasicVal v') = False" |
+"value_ref \<bowtie> (PairVal v1 v2) \<sqsubseteq> (PairVal v1' v2') = (v1 = v1' \<and> v2 = v2')" |
+"value_ref \<bowtie> (PairVal v1 v2) \<sqsubseteq> (SetVal vs') = False" |
+"value_ref \<bowtie> (SetVal vs) \<sqsubseteq> (BasicVal v') = False" |
+"value_ref \<bowtie> (SetVal vs) \<sqsubseteq> (PairVal v1' v2') = False" |
+"value_ref \<bowtie> (SetVal vs) \<sqsubseteq> (SetVal vs') = (vs = vs')"
+
+subsection {* Locale @{text "COMPOSITE_VALUE"} *}
+
+text {* I am not sure yet whether a locale is really necessary here. *}
+
+locale COMPOSITE_VALUE =
+  VALUE "lift_type_rel_composite basic_type_rel"
+    "lift_value_ref_composite basic_value_ref"
+for basic_type_rel :: "'BASIC_VALUE :: BASIC_SORT \<Rightarrow> 'BASIC_TYPE \<Rightarrow> bool" and
+  basic_value_ref :: "'BASIC_VALUE :: BASIC_SORT \<Rightarrow> 'BASIC_VALUE \<Rightarrow> bool"
+begin
+
+subsubsection {* Constructors *}
+
+definition MkInt ::
+  "int \<Rightarrow> 'BASIC_VALUE COMPOSITE_VALUE" where
+"MkInt = INT_SORT_class.MkInt"
+
+definition MkBool ::
+  "bool \<Rightarrow> 'BASIC_VALUE COMPOSITE_VALUE" where
+"MkBool = BOOL_SORT_class.MkBool"
+
+definition MkStr ::
+  "string \<Rightarrow> 'BASIC_VALUE COMPOSITE_VALUE" where
+"MkStr = STRING_SORT_class.MkStr"
+
+definition MkVal ::
+  "'BASIC_VALUE \<Rightarrow>
+   'BASIC_VALUE COMPOSITE_VALUE" where
+"MkVal = BasicVal"
+
+definition MkPair ::
+  "'BASIC_VALUE COMPOSITE_VALUE \<times>
+   'BASIC_VALUE COMPOSITE_VALUE \<Rightarrow>
+   'BASIC_VALUE COMPOSITE_VALUE" where
+"MkPair = PAIR_SORT_class.MkPair"
+
+definition MkSet ::
+  "'BASIC_VALUE COMPOSITE_VALUE set \<Rightarrow>
+   'BASIC_VALUE COMPOSITE_VALUE" where
+"MkSet = SET_SORT_class.MkSet"
+
+text {* Destructors *}
+
+definition DestInt ::
+  "'BASIC_VALUE COMPOSITE_VALUE \<Rightarrow> int" where
+"DestInt = INT_SORT_class.DestInt"
+
+definition DestBool ::
+  "'BASIC_VALUE COMPOSITE_VALUE \<Rightarrow> bool" where
+"DestBool = BOOL_SORT_class.DestBool"
+
+definition DestStr ::
+  "'BASIC_VALUE COMPOSITE_VALUE \<Rightarrow> string" where
+"DestStr = STRING_SORT_class.DestStr"
+
+definition DestVal ::
+  "'BASIC_VALUE COMPOSITE_VALUE \<Rightarrow>
+   'BASIC_VALUE" where
+"DestVal = ValOf"
+
+definition DestPair ::
+  "'BASIC_VALUE COMPOSITE_VALUE \<Rightarrow>
+  ('BASIC_VALUE COMPOSITE_VALUE \<times>
+   'BASIC_VALUE COMPOSITE_VALUE)" where
+"DestPair = PAIR_SORT_class.DestPair"
+
+definition DestSet ::
+  "'BASIC_VALUE COMPOSITE_VALUE \<Rightarrow>
+   'BASIC_VALUE COMPOSITE_VALUE set" where
+"DestSet = SET_SORT_class.DestSet"
+
+subsubsection {* Tests *}
+
+definition IsInt ::
+  "'BASIC_VALUE COMPOSITE_VALUE \<Rightarrow> bool" where
+"IsInt = INT_SORT_class.IsInt"
+
+definition IsBool ::
+  "'BASIC_VALUE COMPOSITE_VALUE \<Rightarrow> bool" where
+"IsBool = BOOL_SORT_class.IsBool"
+
+definition IsStr ::
+  "'BASIC_VALUE COMPOSITE_VALUE \<Rightarrow> bool" where
+"IsStr = STRING_SORT_class.IsStr"
+
+definition IsVal ::
+  "'BASIC_VALUE COMPOSITE_VALUE \<Rightarrow> bool" where
+"IsVal = IsBasicVal"
+
+definition IsPair ::
+  "'BASIC_VALUE COMPOSITE_VALUE \<Rightarrow> bool" where
+"IsPair = PAIR_SORT_class.IsPair"
+
+definition IsSet ::
+  "'BASIC_VALUE COMPOSITE_VALUE \<Rightarrow> bool" where
+"IsSet = SET_SORT_class.IsSet"
+
+subsubsection {* Default Simplificiations *}
+
+declare MkInt_def [simp]
+declare MkBool_def [simp]
+declare MkStr_def [simp]
+declare MkVal_def [simp]
+declare MkPair_def [simp]
+declare MkSet_def [simp]
+
+declare DestInt_def [simp]
+declare DestBool_def [simp]
+declare DestStr_def [simp]
+declare DestVal_def [simp]
+declare DestPair_def [simp]
+declare DestSet_def [simp]
+
+declare IsInt_def [simp]
+declare IsBool_def [simp]
+declare IsStr_def [simp]
+declare IsVal_def [simp]
+declare IsPair_def [simp]
+declare IsSet_def [simp]
+end
+
+subsection {* Theorems *}
+
+theorem lift_type_rel_composite_VALUE [intro!] :
+"\<lbrakk>VALUE basic_type_rel\<rbrakk> \<Longrightarrow>
+ VALUE (lift_type_rel_composite basic_type_rel)"
+apply (simp add: VALUE_def)
+apply (clarify)
+apply (induct_tac t)
+apply (drule_tac x = "BASIC_TYPE" in spec)
+apply (safe)
+apply (rule_tac x = "BasicVal x" in exI)
+apply (simp)
+apply (rule_tac x = "PairVal x xa" in exI)
+apply (auto)
+apply (rule_tac x = "EncSetVal {}" in exI)
+apply (auto)
+done
+
+text {* The following theorem facilitates locale instantiation. *}
+
+theorem TYPED_PRED_inst [intro!, simp] :
+"\<lbrakk>VALUE type_rel\<rbrakk> \<Longrightarrow> COMPOSITE_VALUE type_rel"
+apply (simp add: COMPOSITE_VALUE_def)
+apply (auto)
+done
+end
