theories/generic/utp_function.thy
@@ -1,8 +1,12 @@
-theory utp_gen_fun
-imports utp_gen_pred
+(******************************************************************************)
+(* Title: utp/generic/utp_function.thy                                        *)
+(* Author: Frank Zeyda, University of York                                    *)
+(******************************************************************************)
+theory utp_function
+imports utp_generic_pred
 begin
 
-section {* Functions on Alphabetised Predicates *}
+section {* Functions on Predicates *}
 
 context GEN_PRED
 begin
@@ -12,16 +16,16 @@ types ('a, 'b) ALPHA_FUNCTION =
    ('a, 'b) ALPHA_PREDICATE"
 
 definition WF_ALPHA_FUNCTION :: "('TYPE VAR, 'VALUE) ALPHA_FUNCTION set" where
-"WF_ALPHA_FUNCTION \<equiv>
+"WF_ALPHA_FUNCTION =
  {f . \<forall> p \<in> WF_ALPHA_PREDICATE . f p \<in> WF_ALPHA_PREDICATE}"
 
 definition WF_ALPHA_FUNCTION_OVER ::
   "'TYPE VAR ALPHABET \<Rightarrow> ('TYPE VAR, 'VALUE) ALPHA_FUNCTION set" where
 "\<lbrakk>a \<in> WF_ALPHABET\<rbrakk> \<Longrightarrow>
- WF_ALPHA_FUNCTION_OVER a \<equiv>
+ WF_ALPHA_FUNCTION_OVER a =
  {f . \<forall> p \<in> WF_ALPHA_PREDICATE_OVER a . f p \<in> WF_ALPHA_PREDICATE}"
 
-text {* The following might be useful too, this needs to be explored. *}
+text {* The following could be useful, this still needs to be explored! *}
 
 definition WF_ALPHA_FUNCTION_BETWEEN ::
   "['TYPE VAR ALPHABET, 'TYPE VAR ALPHABET] \<Rightarrow>
@@ -31,26 +35,27 @@ definition WF_ALPHA_FUNCTION_BETWEEN ::
  WF_ALPHA_FUNCTION_BETWEEN a1 a2 \<equiv>
  {f . \<forall> p \<in> WF_ALPHA_PREDICATE_OVER a1 . f p \<in> WF_ALPHA_PREDICATE_OVER a2}"
 
-section {* Semantic Restrictions *}
+section {* Restrictions *}
 
 definition IDEMPOTENT :: "('TYPE VAR, 'VALUE) ALPHA_FUNCTION set" where
-"IDEMPOTENT \<equiv> {f . \<forall> p \<in> WF_ALPHA_PREDICATE . f (f p) = f p}"
+"IDEMPOTENT = {f . \<forall> p \<in> WF_ALPHA_PREDICATE . f (f p) = f p}"
 
 definition IDEMPOTENT_OVER ::
   "'TYPE VAR ALPHABET \<Rightarrow> ('TYPE VAR, 'VALUE) ALPHA_FUNCTION set" where
 "\<lbrakk>a \<in> WF_ALPHABET\<rbrakk> \<Longrightarrow>
- IDEMPOTENT_OVER a \<equiv> {f . \<forall> p \<in> WF_ALPHA_PREDICATE_OVER a . f (f p) = f p}"
+ IDEMPOTENT_OVER a = {f . \<forall> p \<in> WF_ALPHA_PREDICATE_OVER a . f (f p) = f p}"
 
 definition MONOTONIC :: "('TYPE VAR, 'VALUE) ALPHA_FUNCTION set" where
-"MONOTONIC \<equiv>
+"MONOTONIC =
  {f \<in> WF_ALPHA_FUNCTION .
-   \<forall> p1 \<in> WF_ALPHA_PREDICATE .
-   \<forall> p2 \<in> WF_ALPHA_PREDICATE . p1 \<sqsubseteq> p2 \<longrightarrow> f(p1) \<sqsubseteq> f(p2)}"
+   \<forall> a \<in> WF_ALPHABET .
+   \<forall> p1 \<in> WF_ALPHA_PREDICATE_OVER a .
+   \<forall> p2 \<in> WF_ALPHA_PREDICATE_OVER a . p1 \<sqsubseteq> p2 \<longrightarrow> f(p1) \<sqsubseteq> f(p2)}"
 
 definition MONOTONIC_OVER ::
   "'TYPE VAR ALPHABET \<Rightarrow> ('TYPE VAR, 'VALUE) ALPHA_FUNCTION set" where
 "\<lbrakk>a \<in> WF_ALPHABET\<rbrakk> \<Longrightarrow>
- MONOTONIC_OVER a \<equiv>
+ MONOTONIC_OVER a =
  {f \<in> WF_ALPHA_FUNCTION_OVER a .
    \<forall> p1 \<in> WF_ALPHA_PREDICATE_OVER a .
    \<forall> p2 \<in> WF_ALPHA_PREDICATE_OVER a . p1 \<sqsubseteq> p2 \<longrightarrow> f(p1) \<sqsubseteq> f(p2)}"
