theories/generic/utp_gen_value.thy
@@ -1,9 +1,0 @@
-theory utp_gen_value
-imports utp_abstract_value utp_complex_value
-begin
-
-section {* Generic Values *}
-
-text  {* Meta-theory that imports all theories for generic values. *}
-
-end
