theories/generic/utp_generic.thy
@@ -1,13 +1,21 @@
+(******************************************************************************)
+(* Title: utp/generic/utp_generic.thy                                         *)
+(* Author: Frank Zeyda, University of York                                    *)
+(******************************************************************************)
 theory utp_generic
 imports
-  utp_gen_value
-  utp_gen_var
-  utp_gen_pred
-  utp_gen_eval
-  utp_gen_fun
-  utp_gen_bfun
+  utp_name
+  utp_var
+  utp_alphabet
+  utp_abstract_value
+  utp_composite_value
+  utp_generic_pred
+  utp_typed_pred
+  utp_eval_tactic
+  utp_function
+  utp_binding_fun
 begin
 
-text {* Meta-theory that imports all theories and tools for generics. *}
+text {* Meta-theory that imports all theories for generic models. *}
 
 end
