theories/generic/utp_name.thy
@@ -1,0 +1,27 @@
+(******************************************************************************)
+(* Title: utp/generic/utp_name.thy                                            *)
+(* Author: Frank Zeyda, University of York                                    *)
+(******************************************************************************)
+theory utp_name
+imports "../utp_common"
+begin
+
+section {* Variable Names *}
+
+subsection {* Encoding of Subscripts *}
+
+datatype SUBSCRIPT =
+  Sub "nat" | NoSub
+
+subsection {* Encoding of Names *}
+
+record NAME =
+  name_str::"string"
+  dashes::"nat"
+  subscript::"SUBSCRIPT"
+
+subsection {* Restrictions *}
+
+definition NAME_SUBST :: "(NAME \<Rightarrow> NAME) set" where
+"NAME_SUBST = bij"
+end
