theories/theories/utp_all_theories.thy
@@ -1,0 +1,11 @@
+(******************************************************************************)
+(* Title: utp/theories/utp_all_theories.thy                                   *)
+(* Author: Frank Zeyda, University of York                                    *)
+(******************************************************************************)
+theory utp_all_theories
+imports utp_rel
+begin
+
+text {* Meta-theory that imports all UTP theory embeddings. *}
+
+end
