theories/theories/utp_theories.thy
@@ -1,7 +1,0 @@
-theory utp_theories
-imports utp_rel
-begin
-
-text {* Meta-theory that imports all UTP theory mechanisations. *}
-
-end
