theories/theories/utp_theory.thy
@@ -1,0 +1,118 @@
+(******************************************************************************)
+(* Title: utp/theories/utp_theory.thy                                         *)
+(* Author: Frank Zeyda, University of York                                    *)
+(******************************************************************************)
+theory utp_theory
+imports "../GLOBAL" "../generic/utp_generic"
+begin
+
+section {* UTP Theories *}
+
+record ('VAR, 'VALUE) UTP_THEORY =
+  alphabet::"'VAR ALPHABET" ("\<alpha>")
+  healthconds::"('VAR, 'VALUE) ALPHA_FUNCTION set" ("\<H>")
+
+context GEN_PRED
+begin
+definition WF_HEALTH_COND ::
+  "('TYPE VAR) ALPHABET \<Rightarrow>
+   ('TYPE VAR, 'VALUE) ALPHA_FUNCTION set" where
+"a \<in> WF_ALPHABET \<longrightarrow>
+ WF_HEALTH_COND a = {hc . hc \<in> IDEMPOTENT_OVER a}"
+
+(* Should we also require hc \<in> WF_ALPHA_FUNCTION_BETWEEN a a ? *)
+
+definition WF_HEALTH_CONDS ::
+  "('TYPE VAR) ALPHABET \<Rightarrow>
+   ('TYPE VAR, 'VALUE) ALPHA_FUNCTION set set" where
+"a \<in> WF_ALPHABET \<longrightarrow>
+ WF_HEALTH_CONDS a =
+   {hs . finite hs \<and> (\<forall> hc \<in> hs . hc \<in> WF_HEALTH_COND a)}"
+
+definition WF_UTP_THEORY :: "('TYPE VAR, 'VALUE) UTP_THEORY set" where
+"WF_UTP_THEORY =
+   {th . (\<alpha> th) \<in> WF_ALPHABET \<and> (\<H> th) \<in> WF_HEALTH_CONDS (\<alpha> th)}"
+
+subsection {* Theory Operators *}
+
+definition MakeTheory ::
+  "('TYPE VAR) ALPHABET \<Rightarrow>
+   ('TYPE VAR, 'VALUE) ALPHA_FUNCTION set \<Rightarrow>
+   ('TYPE VAR, 'VALUE) UTP_THEORY" where
+"a \<in> WF_ALPHABET \<and>
+ hs \<in> WF_HEALTH_CONDS a \<longrightarrow>
+ MakeTheory a hs = \<lparr>alphabet = a, healthconds = hs\<rparr>"
+
+definition SpecTheory ::
+  "('TYPE VAR, 'VALUE) UTP_THEORY \<Rightarrow>
+   ('TYPE VAR, 'VALUE) ALPHA_FUNCTION set \<Rightarrow>
+   ('TYPE VAR, 'VALUE) UTP_THEORY" where
+"th \<in> WF_UTP_THEORY \<and>
+ hs \<in> WF_HEALTH_CONDS (\<alpha> th) \<longrightarrow>
+ SpecTheory th hs = \<lparr>alphabet = (\<alpha> th), healthconds = (\<H> th) \<union> hs\<rparr>"
+
+subsection {* Theory Predicates *}
+
+definition TheoryPreds ::
+  "('TYPE VAR, 'VALUE) UTP_THEORY \<Rightarrow>
+   ('TYPE VAR, 'VALUE) ALPHA_PREDICATE set" where
+"th \<in> WF_UTP_THEORY \<longrightarrow>
+ TheoryPreds th =
+   {p \<in> WF_ALPHA_PREDICATE_OVER (\<alpha> th) . (\<forall> hc \<in> \<H> th . hc p = p)}"
+
+subsection {* UTP Theory of Predicates *}
+
+definition PredTheory ::
+  "('TYPE VAR) ALPHABET \<Rightarrow>
+   ('TYPE VAR, 'VALUE) UTP_THEORY" where
+"a \<in> WF_ALPHABET \<longrightarrow>
+ PredTheory a = MakeTheory a {}"
+end
+
+subsection {* Theorems *}
+
+context GEN_PRED
+begin
+theorem WF_HEALTH_CONDS_union :
+"\<lbrakk>a \<in> WF_ALPHABET;
+ hs1 \<in> WF_HEALTH_CONDS a;
+ hs2 \<in> WF_HEALTH_CONDS a\<rbrakk> \<Longrightarrow>
+ (hs1 \<union> hs2) \<in> WF_HEALTH_CONDS a"
+apply (simp add: WF_HEALTH_CONDS_def)
+apply (auto)
+done
+
+theorem SpecTheory_closure [simp, intro!] :
+"\<lbrakk>th \<in> WF_UTP_THEORY;
+ hs \<in> WF_HEALTH_CONDS (\<alpha> th)\<rbrakk> \<Longrightarrow>
+ (SpecTheory th hs) \<in> WF_UTP_THEORY"
+apply (simp add: SpecTheory_def)
+apply (simp add: WF_UTP_THEORY_def)
+apply (simp add: WF_HEALTH_CONDS_union)
+done
+
+theorem SpecTheory_alphabet [simp] :
+"\<lbrakk>th \<in> WF_UTP_THEORY;
+ hs \<in> WF_HEALTH_CONDS (\<alpha> th)\<rbrakk> \<Longrightarrow>
+ \<alpha> (SpecTheory th hs) = (\<alpha> th)"
+apply (simp add: SpecTheory_def)
+done
+
+theorem SpecTheory_healthconds [simp] :
+"\<lbrakk>th \<in> WF_UTP_THEORY;
+ hs \<in> WF_HEALTH_CONDS (\<alpha> th)\<rbrakk> \<Longrightarrow>
+ \<H> th \<subseteq> \<H> (SpecTheory th hs)"
+apply (simp add: SpecTheory_def)
+done
+
+theorem SpecTheory_TheoryPreds :
+"\<lbrakk>th \<in> WF_UTP_THEORY;
+ hs \<in> WF_HEALTH_CONDS (\<alpha> th)\<rbrakk> \<Longrightarrow>
+ TheoryPreds (SpecTheory th hs) \<subseteq> TheoryPreds th"
+apply (simp add: TheoryPreds_def)
+apply (safe)
+apply (drule_tac th = "th" and hs = "hs" in SpecTheory_healthconds)
+apply (auto)
+done
+end
+end
